\documentclass[12pt]{article}

\begin{document}

\begin{eqnarray*}
E_i & = & F_\alpha \left( \sum_{j\neq i} \rho_\beta (r_{ij}) \right) + \frac{1}{2} \sum_{j\neq i}\phi_{\alpha\beta}(r_{ij})+ \frac{1}{2} \sum_s (\mu_i^s)^2 + \frac{1}{2} \sum_{s,t} (\lambda_i^{st})^2 - \frac{1}{6} \nu_i^2 \\
%
\mu_i^s & = & \sum_{j\neq i}u_{\alpha\beta}(r_{ij})r_{ij}^s\\
%
\lambda_i^{st} & = & \sum_{j\neq i}w_{\alpha\beta}(r_{ij})r_{ij}^sr_{ij}^t\\
%
\nu_i & = & \sum_s\lambda_i^{ss}
\end{eqnarray*}

\end{document}

