\documentclass[12pt]{article}

\begin{document}

\begin{eqnarray*}
\left\{\begin{array}{l}
\eta_{ij}=\delta_{ij},\xi_{IJ}=0 \\
U_{IJ}\left(r\right)=A_{IJ}\cdot\epsilon_{IJ}\cdot \left(\frac{\sigma_{IJ}}{r}\right)^q\cdot \left[B_{IJ}\cdot \left(\frac{\sigma_{IJ}}{r}\right)^{p-q}-1\right]\cdot exp\left(\frac{\sigma_{IJ}}{r-a_{IJ}\cdot \sigma_{IJ}}\right) \\
V_{IJ}\left(r\right)=\sqrt{\lambda_{IJ}\cdot \epsilon_{IJ}}\cdot exp\left(\frac{\gamma_{IJ}\cdot \sigma_{IJ}}{r-a_{IJ}\cdot \sigma_{IJ}}\right) \\ 
F_{IJ}\left(X\right)=-X \\
P_{IJ}\left(\Delta r\right)=1 \\ 
W_{IJ}\left(r\right)=\sqrt{\lambda_{IJ}\cdot \epsilon_{IJ}}\cdot exp\left(\frac{\gamma_{IJ}\cdot \sigma_{IJ}}{r-a_{IJ}\cdot \sigma_{IJ}}\right) \\
G_{JIK}\left(\theta\right)=\left(cos\theta+\frac{1}{3}\right)^2
\end{array}\right.
\end{eqnarray*} 

\end{document}
