\documentclass[12pt]{article}

\begin{document}

\begin{eqnarray*}
\left\{\begin{array}{l}
\eta_{ij}=\delta_{ij},\xi_{IJ}=1 \\
U_{IJ}\left(r\right)=\frac{D_{e,IJ}}{S_{IJ}-1}\cdot exp\left[-\beta_{IJ}\sqrt{2S_{IJ}\left(r-r_{e,IJ}\right)}\right]\cdot f_{c,IJ}\left(r\right) \\
V_{IJ}\left(r\right)=\frac{S_{IJ}\cdot D_{e,IJ}}{S_{IJ}-1}\cdot exp\left[-\beta_{IJ}\sqrt{\frac{2}{S_{IJ}}\left(r-r_{e,IJ}\right)}\right]\cdot f_{c,IJ}\left(r\right) \\
F_{IJ}\left(X\right)=\left(1+X\right)^{-\frac{1}{2}} \\
P_{IJ}\left(\Delta r\right)=exp\left(2\mu_{IK}\cdot \Delta r\right) \\ 
W_{IJ}\left(r\right)=f_{c,IK}\left(r\right) \\
G_{JIK}\left(\theta\right)=\gamma_{IK}\left[1+\frac{c_{IK}^2}{d_{IK}^2}-\frac{c_{IK}^2}{d_{IK}^2+\left(h_{IK}+cos\theta\right)^2}\right]
\end{array}\right.
\end{eqnarray*} 

\end{document}
