\documentclass[12pt]{article}

\begin{document}

\begin{eqnarray*}
S_{ab} & = & - \left[ m v_a v_b + 
   \frac{1}{2} \sum_{n = 1}^{N_p} (r_{1_a} F_{1_b} + r_{2_a} F_{2_b}) +
   \frac{1}{2} \sum_{n = 1}^{N_b} (r_{1_a} F_{1_b} + r_{2_a} F_{2_b}) + \right. \\
&& \left. \frac{1}{3} \sum_{n = 1}^{N_a} (r_{1_a} F_{1_b} + r_{2_a} F_{2_b} + 
                                           r_{3_a} F_{3_b}) + 
   \frac{1}{4} \sum_{n = 1}^{N_d} (r_{1_a} F_{1_b} + r_{2_a} F_{2_b} + 
				   r_{3_a} F_{3_b} + r_{4_a} F_{4_b}) + \right. \\
&& \left. \frac{1}{4} \sum_{n = 1}^{N_i} (r_{1_a} F_{1_b} + r_{2_a} F_{2_b} + 
                                          r_{3_a} F_{3_b} + r_{4_a} F_{4_b}) +
   {\rm Kspace}(r_{i_a},F_{i_b}) + 
   \sum_{n = 1}^{N_f} r_{i_a} F_{i_b} \right]
\end{eqnarray*}

\end{document}

